Generalize the parse tree property expander a bit
Not sure why the guardedness checker doesn't like transparent definitions...
(I had to recreate expand_forall_parse_of_item' in the middle of the proof)

src/Parsers/ContextFreeGrammarProperties.v
@@ -1,5 +1,6 @@
 (** * Properties about Context Free Grammars *)
 Require Import Parsers.StringLike Parsers.ContextFreeGrammar.
+Require Import Coq.Classes.RelationClasses.
 
 Set Implicit Arguments.
 
@@ -39,46 +40,74 @@ Section cfg.
   End definitions.
 
   Section expand.
-    Context {P P' : String -> String.string -> Type}
-            (f : forall str n, P str n -> P' str n).
+    Context {P P' : String -> String.string -> Type}.
 
     Definition expand_forall_parse_of_item'
+               {str}
                {Forall_parse_of : forall P {str pats} (p : parse_of String G str pats), Type}
-               (expand : forall {str pats p}, @Forall_parse_of P str pats p -> @Forall_parse_of P' str pats p)
-               {str it p}
+               (expand : forall {pats p}, @Forall_parse_of P str pats p -> @Forall_parse_of P' str pats p)
+               (f : forall n, P str n -> P' str n)
+               {it p}
     : @Forall_parse_of_item' P (@Forall_parse_of P) str it p
       -> @Forall_parse_of_item' P' (@Forall_parse_of P') str it p.
     Proof.
       destruct p; simpl.
       { exact (fun x => x). }
       { intro ab.
-        exact (f (fst ab), expand _ _ _ (snd ab)). }
+        exact (f _ (fst ab), expand _ _ (snd ab)). }
     Defined.
 
     Global Arguments expand_forall_parse_of_item' : simpl never.
 
-    Fixpoint expand_forall_parse_of {str pats} {p : parse_of String G str pats}
+    Fixpoint expand_forall_parse_of
+             str
+             (f : forall str', str' ≤s str -> forall n, P str' n -> P' str' n)
+             pats (p : parse_of String G str pats)
+             {struct p}
     : Forall_parse_of P p -> Forall_parse_of P' p
-      := match p return Forall_parse_of P p -> Forall_parse_of P' p with
-           | ParseHead str pat pats p'
-             => @expand_forall_parse_of_production _ _ p'
-           | ParseTail _ _ _ p'
-             => @expand_forall_parse_of _ _ p'
-         end
-    with expand_forall_parse_of_production {str pat} {p : parse_of_production String G str pat}
-         : Forall_parse_of_production P p -> Forall_parse_of_production P' p
-         := match p return Forall_parse_of_production P p -> Forall_parse_of_production P' p with
-              | ParseProductionNil => fun x => x
-              | ParseProductionCons str pat strs pats p' p''
-                => fun ab => (expand_forall_parse_of_item' (@expand_forall_parse_of) (fst ab),
-                              expand_forall_parse_of_production (snd ab))
-            end.
+    with expand_forall_parse_of_production
+           str
+           (f : forall str', str' ≤s str -> forall n, P str' n -> P' str' n)
+           pat (p : parse_of_production String G str pat)
+           {struct p}
+         : Forall_parse_of_production P p -> Forall_parse_of_production P' p.
+    Proof.
+      { exact (match p in parse_of _ _ str' pats'
+                     return (forall str'', str'' ≤s str' -> forall n, P str'' n -> P' str'' n)
+                            -> Forall_parse_of P p -> Forall_parse_of P' p
+               with
+                 | ParseHead _ _ _ p'
+                   => fun f' => @expand_forall_parse_of_production _ f' _ p'
+                 | ParseTail _ _ _ p'
+                   => fun f' => @expand_forall_parse_of _ f' _ p'
+               end f). }
+      { refine (match p in parse_of_production _ _ str' pats'
+                      return (forall str'', str'' ≤s str' -> forall n, P str'' n -> P' str'' n)
+                             -> Forall_parse_of_production P p -> Forall_parse_of_production P' p
+                with
+                  | ParseProductionNil => fun _ x => x
+                  | ParseProductionCons str' pat strs' pats p' p''
+                    => fun f' ab
+                       => (_ : Forall_parse_of_item' _ (@Forall_parse_of _) _,
+                           expand_forall_parse_of_production
+                             _
+                             (fun str'' pf'' => f' str'' (transitivity pf'' (str_le2_append _ _ _)))
+                             _ _
+                             (snd ab))
+                end f).
+        destruct p'; simpl.
+        { exact tt. }
+        { refine (f' _ (str_le1_append _ _ _) _ (fst (fst ab)),
+                  expand_forall_parse_of _ _ _ _ (snd (fst ab))).
+          intros ??; apply f'.
+          etransitivity; [ eassumption | exact (str_le1_append _ _ _) ]. } }
+    Defined.
 
     Global Arguments expand_forall_parse_of : simpl never.
     Global Arguments expand_forall_parse_of_production : simpl never.
 
-    Definition expand_forall_parse_of_item {str it} {p : parse_of_item String G str it}
-      := @expand_forall_parse_of_item' _ (@expand_forall_parse_of) str it p.
+    Definition expand_forall_parse_of_item {str} f {it} {p : parse_of_item String G str it}
+      := @expand_forall_parse_of_item' str _ (@expand_forall_parse_of str f) (f _ (reflexivity _)) it p.
 
     Global Arguments expand_forall_parse_of_item : simpl never.
   End expand.
